# Explanation

[4, 1, 2]
[1, 2, 3, 4]

For the second array, NGE(1) = 2, NGE(2) = 3, NGE(3) = 4, NGE(4) = -1
Note that NGE is the first element that it encounters.

Therefore, for the answer to the first array is

[NGE(4), NGE(1), NGE(2)] = [-1, 2, 3]

# solve1.cc

17 / 17 test cases passed.
Status: Accepted
Runtime: 126 ms

Your runtime beats 55.74% of javascript submissions.

# solve2.cc

17 / 17 test cases passed.
Status: Accepted
Runtime: 182 ms

Your runtime beats 15.08% of javascript submissions.


